Problem with a mutable ref

CoqOfRust/revm/revm_interpreter/instructions/links/bitwise.v
@@ -1,6 +1,7 @@
 Require Import CoqOfRust.CoqOfRust.
 Require Import CoqOfRust.links.lib.
 Require Import CoqOfRust.links.M.
+Require Import core.links.intrinsics.
 Require Import revm.revm_context_interface.links.host.
 Require revm.links.dependencies.
 Import revm.links.dependencies.ruint.
@@ -11,69 +12,64 @@ Require Import revm.revm_interpreter.instructions.bitwise.
 
 Import Run.
 (*
-pub fn add<WIRE: InterpreterTypes, H: Host + ?Sized>(
-    interpreter: &mut Interpreter<WIRE>,
-    _host: &mut H,
-)
-
 pub fn lt<WIRE: InterpreterTypes, H: Host + ?Sized>(
     interpreter: &mut Interpreter<WIRE>,
     _host: &mut H,
 )
 *)
 
-Definition run_lt
+Ltac solve_one_branch e :=
+  constructor;
+  cbn;
+  eapply Run.Rewrite; [
+    repeat erewrite IsTraitAssociatedType_eq by apply e;
+    reflexivity
+  |
+  ];
+  run_symbolic.
+
+Instance run_lt
     {WIRE H : Set} `{Link WIRE} `{Link H}
     {WIRE_types : InterpreterTypes.Types.t} `{InterpreterTypes.Types.AreLinks WIRE_types}
     (run_InterpreterTypes_for_WIRE : InterpreterTypes.Run WIRE WIRE_types)
     (interpreter : Ref.t Pointer.Kind.MutRef (Interpreter.t WIRE WIRE_types))
     (_host : Ref.t Pointer.Kind.MutRef H) :
-  {{
-    instructions.bitwise.lt [] [ Φ WIRE; Φ H ] [ φ interpreter; φ _host ] 🔽
-    unit
-  }}.
+  Run.Trait
+    instructions.bitwise.lt [] [ Φ WIRE; Φ H ] [ φ interpreter; φ _host ]
+    unit.
 Proof.
-  run_symbolic.
+  constructor.
+  cbn.
   eapply Run.Rewrite. {
     repeat erewrite IsTraitAssociatedType_eq by apply run_InterpreterTypes_for_WIRE.
     reflexivity.
   }
-  run_symbolic_let. {
-    run_symbolic.
-    destruct run_InterpreterTypes_for_WIRE.
-    destruct run_LoopControl_for_Control.
-    destruct gas as [gas [H_gas run_gas]].
-    destruct set_instruction_result as [set_instruction_result [H_set_instruction_result run_set_instruction_result]].
-    run_symbolic.
-    run_symbolic_closure. {
-      apply Impl_Gas.run_record_cost.
-    }
-    intros []; run_symbolic.
-    run_symbolic_are_equal_bool; run_symbolic.
-  }
-  intros [|[]]; run_symbolic.
   destruct run_InterpreterTypes_for_WIRE.
   destruct run_StackTrait_for_Stack.
   destruct popn_top as [popn_top [H_popn_top run_popn_top]].
-  run_symbolic.
-  run_symbolic_let. {
-    run_symbolic.
-    eapply Run.CallPrimitiveGetTraitMethod.
-    { eapply IsTraitMethod.Defined.
-       - specialize (Impl_PartialOrd_for_Uint.Implements
-       (Value.Integer IntegerKind.Usize 256)
-       (Value.Integer IntegerKind.Usize 4)).
-       intros.
-       unfold Impl_PartialOrd_for_Uint.Self in H3.
-       apply H3 with (trait_tys := [Ty.apply (Ty.path "ruint::Uint")
+  destruct run_LoopControl_for_Control.
+  destruct gas as [gas [H_gas run_gas]].
+  destruct set_instruction_result as [set_instruction_result [H_set_instruction_result run_set_instruction_result]].
+  run_symbolic. {
+    repeat solve_one_branch run_InterpreterTypes_for_WIRE.
+  }
+  eapply Run.CallPrimitiveGetTraitMethod.
+  - eapply IsTraitMethod.Defined.
+    + specialize (Impl_PartialOrd_for_Uint.Implements
+    (Value.Integer IntegerKind.Usize 256)
+    (Value.Integer IntegerKind.Usize 4)).
+      intros.
+      unfold Impl_PartialOrd_for_Uint.Self in H3.
+      apply H3 with (trait_tys := [Ty.apply (Ty.path "ruint::Uint")
         [Value.Integer IntegerKind.Usize 256;
          Value.Integer IntegerKind.Usize 4] []]).
-      - simpl.
-        reflexivity.
-    }
-    run_symbolic.
-    
-  }
-  intros [|[]]; run_symbolic.
+    + simpl.
+      reflexivity.
+  - run_symbolic.
+    + 
+
+Qed.
+  
+  
 
 
